---
title: "sta602_hw5"
author: "Dingyan Zhong"
date: "2023-02-08"
output: pdf_document
---
## Question 1
### (a)
Since Y follows a binomial distribution,
$$
\begin{aligned}
  &p(Y=y|\theta) = \binom{n}{y}\theta^y(1-\theta)^{n-y}\\
  \Rightarrow &\ln(p(Y=y|\theta)) = \ln\binom{n}{y}+y\ln\theta+(n-y)\ln(1-\theta)\\
\end{aligned}
$$
Therefore,
$$
\frac{\partial \ln p(Y=y|\theta)}{\partial \theta} = \frac{y}{\theta}+\frac{n-y}{\theta-1}
$$

$$
\frac{\partial^2 \ln p(Y=y|\theta)}{\partial \theta^2} = -\frac{y}{\theta^2}-\frac{n-y}{(\theta-1)^2}
$$
Then, we have
$$
\begin{aligned}
  I(\theta) &= \sum_{y=0}^n (\frac{y}{\theta^2}+\frac{n-y}{(\theta-1)^2})p(Y=y|\theta)\\
            &= \left(\frac{1}{\theta^2}-\frac{1}{(\theta-1)^2}\right)\sum_{y=0}^n yp(Y=y|\theta)
               +\frac{n}{(\theta-1)^2}\sum_{i=0}^np(Y=y|\theta)\\
            &= \left(\frac{1}{\theta^2}-\frac{1}{(\theta-1)^2}\right)n\theta + \frac{n}{(\theta-1)^2}\\
            &= \frac{n}{\theta(1-\theta)}
\end{aligned}
$$

Eventually,
$$
\begin{aligned}
    p_{J}(\theta) &\propto \sqrt{\frac{n}{\theta(1-\theta)}}\\
                  &\propto \theta^{-\frac{1}{2}}(1-\theta)^{-\frac{1}{2}}\\
                  &\propto Beta(\frac{1}{2},\frac{1}{2})\\
\end{aligned}
$$

### (b)
Similar to part(a),
$$
  \ln p(Y=y|\psi) = \ln \binom{n}{y}+\psi y-n\ln(1+e^{\psi})
$$
Therefore,
$$
\begin{aligned}
  \frac{\partial \ln p(Y=y|\psi)}{\partial \psi} &= y -n\left(1-\frac{1}{1+e^{\psi}}\right)\\
  \frac{\partial^2 \ln p(Y=y|\psi)}{\partial \psi^2} &= -\frac{ne^{\psi}}{(1+e^{\psi})^2}\\
\end{aligned}
$$
Hence,
$$
I(\theta) = \sum_{y=0}^n\frac{ne^{\psi}}{(1+e^{\psi})^2}p(Y=y|\psi) = \frac{ne^{\psi}}{(1+e^{\psi})^2}
$$
and

$$
p_J(\psi) \propto \sqrt{\frac{ne^{\psi}}{(1+e^{\psi})^2}} \propto \frac{e^{\psi/2}}{1+e^{\psi}}
$$
### (c)
From the problem description, we know
$$
  \theta = \frac{e^\psi}{1+e^\psi}
$$
By Change of Variable Theorem,
$$
\begin{aligned}
p_J(\psi) &\propto \left(\frac{e^\psi}{1+e^\psi}\right)^{-1/2}\left(\frac{1}{1+e^\psi}\right)^{-1/2}\left|\frac{d\theta}{d \psi}\right|\\
          &\propto \left(\frac{e^\psi}{1+e^\psi}\right)^{-1/2}\left(\frac{1}{1+e^\psi}\right)^{-1/2}\frac{e^\psi}{(1+e^\psi)^2}\\
          &\propto \frac{e^{\psi/2}}{1+e^{\psi}}
\end{aligned}
$$

```{r}


```